src/compiler_generic/toy_example/embedding/OCL_compiler_core.thy
@@ -44,17 +44,11 @@
 header{* Part ... *}
 
 theory  OCL_compiler_core
-imports "core/OCL_compiler_floor1_enum"
-        "core/OCL_compiler_floor1_infra"
-        "core/OCL_compiler_floor1_astype"
-        "core/OCL_compiler_floor1_istypeof"
-        "core/OCL_compiler_floor1_iskindof"
-        "core/OCL_compiler_floor1_allinst"
+imports "core/OCL_compiler_floor1_infra"
         "core/OCL_compiler_floor1_access"
         "core/OCL_compiler_floor1_examp"
         "core/OCL_compiler_floor2_examp"
         "core/OCL_compiler_floor1_ctxt"
-        "core/OCL_compiler_floor2_ctxt"
 begin
 
 section{* Translation of AST *}
@@ -88,299 +82,38 @@ definition "txt''a s = txt (\<lambda> Gen_only_design \<Rightarrow> \<open>\<clo
 definition' thy_class ::
   (* polymorphism weakening needed by code_reflect *)
   "_ h_theory" where \<open>thy_class =
-  (let subsection_def = subsection \<open>Definition\<close>
-     ; subsection_cp = subsection \<open>Context Passing\<close>
-     ; subsection_exec = subsection \<open>Execution with Invalid or Null as Argument\<close>
-     ; subsection_defined = subsection \<open>Validity and Definedness Properties\<close>
-     ; subsection_up = subsection \<open>Up Down Casting\<close>
-     ; subsection_const = subsection \<open>Const\<close> in
-  (Hol_theory_ext o L.flatten)
-          [ [ print_infra_enum_synonym ]
-            , [ txt''d [ \<open>
-   \label{ex:employee-design:uml} \<close> ]
-            , txt''a [ \<open>
-   \label{ex:employee-analysis:uml} \<close> ]
-            , section \<open>Introduction\<close>
-            , txt'' [ \<open>
-
-  For certain concepts like classes and class-types, only a generic
-  definition for its resulting semantics can be given. Generic means,
-  there is a function outside HOL that ``compiles'' a concrete,
-  closed-world class diagram into a ``theory'' of this data model,
-  consisting of a bunch of definitions for classes, accessors, method,
-  casts, and tests for actual types, as well as proofs for the
-  fundamental properties of these operations in this concrete data
-  model. \<close> ]
-            , txt'' [ \<open>
-   Such generic function or ``compiler'' can be implemented in
-  Isabelle on the ML level.  This has been done, for a semantics
-  following the open-world assumption, for UML 2.0
-  in~\cite{brucker.ea:extensible:2008-b, brucker:interactive:2007}. In
-  this paper, we follow another approach for UML 2.4: we define the
-  concepts of the compilation informally, and present a concrete
-  example which is verified in Isabelle/HOL. \<close> ]
-            , subsection \<open>Outlining the Example\<close>
-            , txt''d [ \<open>
-   We are presenting here a ``design-model'' of the (slightly
-modified) example Figure 7.3, page 20 of
-the OCL standard~\cite{omg:ocl:2012}. To be precise, this theory contains the formalization of
-the data-part covered by the UML class model (see \autoref{fig:person}):\<close> ]
-            , txt''a [ \<open>
-   We are presenting here an ``analysis-model'' of the (slightly
-modified) example Figure 7.3, page 20 of
-the OCL standard~\cite{omg:ocl:2012}.
-Here, analysis model means that associations
-were really represented as relation on objects on the state---as is
-intended by the standard---rather by pointers between objects as is
-done in our ``design model'' (see \autoref{ex:employee-design:uml}).
-To be precise, this theory contains the formalization of the data-part
-covered by the UML class model (see \autoref{fig:person-ana}):\<close> ]
-            , txt''d [ \<open>
-
-\begin{figure}
-  \centering\scalebox{.3}{\includegraphics{figures/person.png}}%
-  \caption{A simple UML class model drawn from Figure 7.3,
-  page 20 of~\cite{omg:ocl:2012}. \label{fig:person}}
-\end{figure}
-\<close> ]
-            , txt''a [ \<open>
-
-\begin{figure}
-  \centering\scalebox{.3}{\includegraphics{figures/person.png}}%
-  \caption{A simple UML class model drawn from Figure 7.3,
-  page 20 of~\cite{omg:ocl:2012}. \label{fig:person-ana}}
-\end{figure}
-\<close> ]
-            , txt'' [ \<open>
-   This means that the association (attached to the association class
-\inlineocl{EmployeeRanking}) with the association ends \inlineocl+boss+ and \inlineocl+employees+ is implemented
-by the attribute  \inlineocl+boss+ and the operation \inlineocl+employees+ (to be discussed in the OCL part
-captured by the subsequent theory).
-\<close> ]
-            , section \<open>Example Data-Universe and its Infrastructure\<close>
-            (*, txt'' [ \<open>
-   Ideally, the following is generated automatically from a UML class model.  \<close> ]
-            *), txt'' [ \<open>
-   Our data universe  consists in the concrete class diagram just of node's,
-and implicitly of the class object. Each class implies the existence of a class
-type defined for the corresponding object representations as follows: \<close> ]
-            (*, print_latex_infra_datatype_class*)
-            , print_infra_datatype_class
-            , txt'' [ \<open>
-   Now, we construct a concrete ``universe of OclAny types'' by injection into a
-sum type containing the class types. This type of OclAny will be used as instance
-for all respective type-variables. \<close> ]
-            , print_infra_datatype_universe
-            , txt'' [ \<open>
-   Having fixed the object universe, we can introduce type synonyms that exactly correspond
-to OCL types. Again, we exploit that our representation of OCL is a ``shallow embedding'' with a
-one-to-one correspondance of OCL-types to types of the meta-language HOL. \<close> ]
-            , print_infra_type_synonym_class
-            , print_infra_type_synonym_class_higher
-            , print_infra_type_synonym_class_rec
-            , print_infra_enum_syn
-            (*, txt'' [ \<open>
-   Just a little check: \<close> ]
-            *), txt'' [ \<open>
-   To reuse key-elements of the library like referential equality, we have
-to show that the object universe belongs to the type class ``oclany,'' \ie,
- each class type has to provide a function @{term oid_of} yielding the object id (oid) of the object. \<close> ]
-            , print_infra_instantiation_class
-            , print_infra_instantiation_universe
-
-            , section \<open>Instantiation of the Generic Strict Equality\<close>
-            , txt'' [ \<open>
-   We instantiate the referential equality
-on @{text "Person"} and @{text "OclAny"} \<close> ]
-            , print_instantia_def_strictrefeq
-            , print_instantia_lemmas_strictrefeq
-            , txt'' [ \<open>
-   For each Class \emph{C}, we will have a casting operation \inlineocl{.oclAsType($C$)},
-   a test on the actual type \inlineocl{.oclIsTypeOf($C$)} as well as its relaxed form
-   \inlineocl{.oclIsKindOf($C$)} (corresponding exactly to Java's \verb+instanceof+-operator.
-\<close> ]
-            , txt'' [ \<open>
-   Thus, since we have two class-types in our concrete class hierarchy, we have
-two operations to declare and to provide two overloading definitions for the two static types.
-\<close> ] ]
-
-          , L.flatten (L.map (\<lambda>(title, body_def, body_cp, body_exec, body_defined, body_up, body_const).
-              section title # L.flatten [ subsection_def # body_def
-                                      , subsection_cp # body_cp
-                                      , subsection_exec # body_exec
-                                      , subsection_defined # body_defined
-                                      , subsection_up # body_up
-                                      , subsection_const # body_const ])
-          [ (\<open>OclAsType\<close>,
-            [ print_astype_consts
-            , print_astype_class
-            , print_astype_from_universe
-            , print_astype_lemmas_id ]
-            , [ print_astype_lemma_cp
-            , print_astype_lemmas_cp ]
-            , [ print_astype_lemma_strict
-            , print_astype_lemmas_strict ]
-            , [ print_astype_defined ]
-            , [ print_astype_up_d_cast0
-            , print_astype_up_d_cast
-            , print_astype_d_up_cast ]
-            , [ print_astype_lemma_const
-              , print_astype_lemmas_const ])
-
-          , (\<open>OclIsTypeOf\<close>,
-            [ print_istypeof_consts
-            , print_istypeof_class
-            , print_istypeof_from_universe
-            , print_istypeof_lemmas_id ]
-            , [ print_istypeof_lemma_cp
-            , print_istypeof_lemmas_cp ]
-            , [ print_istypeof_lemma_strict
-            , print_istypeof_lemmas_strict ]
-            , [ print_istypeof_defined
-            , print_istypeof_defined' ]
-            , [ print_istypeof_up_larger
-            , print_istypeof_up_d_cast ]
-            , [])
-
-          , (\<open>OclIsKindOf\<close>,
-            [ print_iskindof_consts
-            , print_iskindof_class
-            , print_iskindof_from_universe
-            , print_iskindof_lemmas_id ]
-            , [ print_iskindof_lemma_cp
-            , print_iskindof_lemmas_cp ]
-            , [ print_iskindof_lemma_strict
-            , print_iskindof_lemmas_strict ]
-            , [ print_iskindof_defined
-            , print_iskindof_defined' ]
-            , [ print_iskindof_up_eq_asty
-            , print_iskindof_up_larger
-            , print_iskindof_up_istypeof_unfold
-            , print_iskindof_up_istypeof
-            , print_iskindof_up_d_cast ]
-            , []) ])
-
-          , [ section \<open>OclAllInstances\<close>
-            , txt'' [ \<open>
-   To denote OCL-types occuring in OCL expressions syntactically---as, for example,  as
-``argument'' of \inlineisar{oclAllInstances()}---we use the inverses of the injection
-functions into the object universes; we show that this is sufficient ``characterization.'' \<close> ]
-            , print_allinst_def_id
-            , print_allinst_lemmas_id
-            , print_allinst_astype
-            , print_allinst_exec
-            , subsection \<open>OclIsTypeOf\<close>
-            , print_allinst_istypeof_pre
-            , print_allinst_istypeof
-            , subsection \<open>OclIsKindOf\<close>
-            , print_allinst_iskindof_eq
-            , print_allinst_iskindof_larger
-
-            , section \<open>The Accessors\<close>
-            , txt''d [ \<open>
-  \label{sec:edm-accessors}\<close> ]
-            , txt''a [ \<open>
-  \label{sec:eam-accessors}\<close> ]
-            (*, txt'' [ \<open>
-   Should be generated entirely from a class-diagram. \<close> ]
-            *), subsection_def
-            , txt''a [ \<open>
-   We start with a oid for the association; this oid can be used
-in presence of association classes to represent the association inside an object,
-pretty much similar to the \inlineisar+Employee_DesignModel_UMLPart+, where we stored
-an \verb+oid+ inside the class as ``pointer.'' \<close> ]
-            , print_access_oid_uniq_ml
-            , print_access_oid_uniq
-            , txt''a [ \<open>
-   From there on, we can already define an empty state which must contain
-for $\mathit{oid}_{Person}\mathcal{BOSS}$ the empty relation (encoded as association list, since there are
-associations with a Sequence-like structure).\<close> ]
-            , print_access_eval_extract
-            , txt''a [ \<open>
-   The @{text pre_post}-parameter is configured with @{text fst} or
-@{text snd}, the @{text to_from}-parameter either with the identity @{term id} or
-the following combinator @{text switch}: \<close> ]
-            , print_access_choose_ml
-            , print_access_choose
-            , print_access_deref_oid
-            , print_access_deref_assocs
-            , txt'' [ \<open>
-   pointer undefined in state or not referencing a type conform object representation \<close> ]
-            , print_access_select
-            , print_access_select_obj
-            , print_access_dot_consts
-            , print_access_dot
-            , print_access_dot_lemmas_id
-            , subsection_cp
-            , print_access_dot_cp_lemmas
-            , print_access_dot_lemma_cp
-            , print_access_dot_lemmas_cp
-            , subsection_exec
-            , print_access_lemma_strict
-            , subsection \<open>Representation in States\<close>
-            , print_access_def_mono
-            , print_access_is_repr
-            , print_access_repr_allinst
-
-            , section \<open>A Little Infra-structure on Example States\<close>
-            , txt''d [ \<open>
-
-The example we are defining in this section comes from the figure~\ref{fig:edm1_system-states}.
-\begin{figure}
-\includegraphics[width=\textwidth]{figures/pre-post.pdf}
-\caption{(a) pre-state $\sigma_1$ and
-  (b) post-state $\sigma_1'$.}
-\label{fig:edm1_system-states}
-\end{figure}
-\<close> ]
-            , txt''a [ \<open>
-
-The example we are defining in this section comes from the figure~\ref{fig:eam1_system-states}.
-\begin{figure}
-\includegraphics[width=\textwidth]{figures/pre-post.pdf}
-\caption{(a) pre-state $\sigma_1$ and
-  (b) post-state $\sigma_1'$.}
-\label{fig:eam1_system-states}
-\end{figure}
-\<close> ]
-            , print_examp_def_st_defs
-            , print_astype_lemmas_id2 ] ])\<close>
+  Hol_theory_ext
+          [ print_infra_datatype_class
+          , print_infra_datatype_universe
+          , print_infra_type_synonym_class_higher
+          , print_access_oid_uniq
+          , print_access_choose ]\<close>
 
 definition "thy_enum_flat = Hol_theory_ext []"
-definition "thy_enum = Hol_theory_ext [ print_enum ]"
+definition "thy_enum = Hol_theory_ext []"
 definition "thy_class_synonym = Hol_theory_ext []"
 definition "thy_class_flat = Hol_theory_ext []"
 definition "thy_association = Hol_theory_ext []"
 definition "thy_instance = Hol_theory_ext 
-                             [ print_examp_instance_defassoc_typecheck_var
-                             , print_examp_instance_defassoc
-                             , print_examp_instance
-                             , print_examp_instance_defassoc_typecheck ]"
-definition "thy_def_base_l = Hol_theory_ext [ print_examp_oclbase ]"
+                             [ print_examp_instance_defassoc
+                             , print_examp_instance ]"
+definition "thy_def_base_l = Hol_theory_ext []"
 definition "thy_def_state = (\<lambda> Floor1 \<Rightarrow> Hol_theory_ext 
                                            [ OCL_compiler_floor1_examp.print_examp_def_st_typecheck_var
                                            , OCL_compiler_floor1_examp.print_examp_def_st1 ]
                              | Floor2 \<Rightarrow> Hol_theory_locale
                                            OCL_compiler_floor2_examp.print_examp_def_st_locale
                                            [ OCL_compiler_floor2_examp.print_examp_def_st2
-                                           , OCL_compiler_floor2_examp.print_examp_def_st_dom
-                                           , OCL_compiler_floor2_examp.print_examp_def_st_dom_lemmas
-                                           , OCL_compiler_floor2_examp.print_examp_def_st_perm
-                                           , OCL_compiler_floor2_examp.print_examp_def_st_allinst
-                                           , OCL_compiler_floor2_examp.print_examp_def_st_defassoc_typecheck ])"
+                                           , OCL_compiler_floor2_examp.print_examp_def_st_perm ])"
 definition "thy_def_pre_post = (\<lambda> Floor1 \<Rightarrow> Hol_theory_ext 
                                               [ OCL_compiler_floor1_examp.print_pre_post ]
                                 | Floor2 \<Rightarrow> Hol_theory_locale
                                               OCL_compiler_floor2_examp.print_pre_post_locale
-                                              [ OCL_compiler_floor2_examp.print_pre_post_interp
-                                              , OCL_compiler_floor2_examp.print_pre_post_wff
-                                              , OCL_compiler_floor2_examp.print_pre_post_where ])"
+                                              [ OCL_compiler_floor2_examp.print_pre_post_interp ])"
 definition "thy_ctxt = (\<lambda> Floor1 \<Rightarrow> Hol_theory_ext 
                                       [ OCL_compiler_floor1_ctxt.print_ctxt ]
                         | Floor2 \<Rightarrow> Hol_theory_ext 
-                                      [ OCL_compiler_floor2_ctxt.print_ctxt_pre_post
-                                      , OCL_compiler_floor2_ctxt.print_ctxt_inv
-                                      , OCL_compiler_floor2_ctxt.print_ctxt_thm ])"
+                                      [])"
 definition "thy_flush_all = Hol_theory_ext []"
 (* NOTE typechecking functions can be put at the end, however checking already defined constants can be done earlier *)
 
