src/compiler_generic/toy_example/embedding/core/OCL_compiler_core_init.thy
@@ -44,7 +44,7 @@
 header{* Part ... *}
 
 theory  OCL_compiler_core_init
-imports "../meta/OCL_compiler_meta_META"
+imports "../meta_toy/OCL_compiler_meta_META"
 begin
 
 section{* Preliminaries Compiler *}
